LeanSubst/Laws.lean
@@ -1,65 +1,14 @@
 
 import LeanSubst.Basic
 import LeanSubst.Ops
+import LeanSubst.Class
+import LeanSubst.Types.Nat
+import LeanSubst.Types.List
 
 namespace LeanSubst
 
 universe u1 u2 u3
 variable {S : Type u1} {T : Type u2} {U : Type u3}
-
-class RenMapId (S : Type u1) (T : Type u2) [RenMap S T] where
-  apply_id {s : S} : s⟨.id T⟩ = s
-
-class RenMapCompose (S : Type u1) (T : Type u2) [RenMap S T] where
-  apply_compose {s : S} {r1 r2 : Ren T} : s⟨r1⟩⟨r2⟩ = s⟨r1 ∘ r2⟩
-
-@[simp]
-theorem Ren.apply_id [RenMap S T] [RenMapId S T] {s : S} : s⟨id T⟩ = s := RenMapId.apply_id
-
-@[simp, grind =]
-theorem Ren.apply_compose [RenMap S T] [RenMapCompose S T] {s : S} {r1 r2 : Ren T}
-  : s⟨r1⟩⟨r2⟩ = s⟨r1 ∘ r2⟩
-:= RenMapCompose.apply_compose
-
-instance (priority := high) [RenMap T T] [RenMapId T T] : RenMapId (Action T) T where
-  apply_id := by intro s; cases s <;> simp
-
-instance [RenMap S T] [RenMapId S T] : RenMapId (Action S) T where
-  apply_id := by intro s; cases s <;> simp
-
-instance (priority := high) [RenMap T T] [RenMapCompose T T] : RenMapCompose (Action T) T where
-  apply_compose := by intro s; cases s <;> simp
-
-instance [RenMap S T] [RenMapCompose S T] : RenMapCompose (Action S) T where
-  apply_compose := by intro s; cases s <;> simp
-
-class SubstMapId (S : Type u1) (T : Type u2) [SubstMap S T] where
-  apply_id {s : S} : s[.id T] = s
-
-class SubstMapStable (S : Type u1) (T : Type u2) [RenMap S T] [SubstMap S T] where
-  apply_stable (r : Ren T) (σ : Subst T) : r.to = σ -> rmap (S := S) r = smap σ
-
-class SubstMapRenComposeLeft (S : Type u1) (T : Type u2) [RenMap S T] [SubstMap S T] where
-  apply_ren_compose_left {s : S} {r : Ren T} {τ : Subst T} : s⟨r⟩[τ] = s[r ∘ τ]
-
-class SubstMapRenComposeRight (T : Type u2) [RenMap T T] [SubstMap T T] where
-  apply_ren_compose_right {t : T} {r : Ren T} {σ : Subst T} : t[σ]⟨r⟩ = t[σ ∘ r]
-
-class SubstMapCompose (S : Type u1) (T : Type u2) [SubstMap S T] [SubstMap T T] where
-  apply_compose {s : S} {σ τ : Subst T} : s[σ][τ] = s[σ ∘ τ]
-
-class SubstMapRenCommute (S : Type u1) (T : Type u2) [RenMap S S] [SubstMap S T] where
-  apply_ren_commute {s : S} (r : Ren S) (τ : Subst T) : s⟨r⟩[τ] = s[τ]⟨r⟩
-
-class SubstMapHetCompose (S : Type u1) (T : Type u2) [SubstMap S S] [SubstMap S T] where
-  apply_hcompose {s : S} {σ : Subst S} {τ : Subst T} : s[σ][τ] = s[τ][σ ◾ τ]
-
-namespace Subst
-  export SubstMapStable (apply_stable)
-  export SubstMapRenComposeLeft (apply_ren_compose_left)
-  export SubstMapRenComposeRight (apply_ren_compose_right)
-  export SubstMapRenCommute (apply_ren_commute)
-end Subst
 
 @[grind <-]
 theorem Ren.lift_eq_from_eq [RenMap T T] {r : Ren T} {σ : Subst T}
@@ -79,47 +28,67 @@ namespace Subst
     @[simp, grind =]
     theorem I_lift [RenMap T T] {k} : +0.lift k = id T := by
       funext; case _ x =>
-      cases x; all_goals (simp [Subst.lift, Subst.id])
+      cases x; all_goals (simp [lift, id, act])
       grind
 
     @[simp, grind =]
     theorem rewrite2 [SubstMap T T] {σ : Subst T} : +0 ∘ σ = σ := by
       funext; case _ x =>
-      unfold Subst.compose; simp [Subst.id]
+      simp [compose, id, act]
 
     @[simp, grind =]
-    theorem rewrite3_replace [SubstMap T T] {σ τ : Subst T} {s : T}
-      : (su s :: σ) ∘ τ = su s[τ] :: (σ ∘ τ)
+    theorem rewrite3_cons [SubstMap T T] {σ τ : Subst T} {a : Action T}
+      : (a :: σ) ∘ τ = a[τ] :: (σ ∘ τ)
     := by
-      simp [Subst.cons, Subst.compose]
+      simp [cons, compose]
       funext; case _ x =>
-      cases x; all_goals simp
+      cases x; all_goals simp [act]
 
     @[simp, grind =]
-    theorem rewrite3_rename [SubstMap T T] {s} {σ τ : Subst T}
-      : (re s :: σ) ∘ τ = (τ.act s) :: (σ ∘ τ)
+    theorem rewrite3_cons_ren [RenMap T T] [SubstMap T T] {σ : Subst T} {r : Ren T} {x : Nat}
+      : (re x :: σ) ∘ r = re (r.act x) :: (σ ∘ r)
     := by
-      simp [Subst.cons, Subst.compose]
+      simp [cons, compose_ren_right]
       funext; case _ x =>
-      cases x; all_goals simp
+      cases x; all_goals simp [act]
 
     @[simp, grind =]
-    theorem rewrite4 [SubstMap T T]  {s} {σ : Subst T} : +1 ∘ (s :: σ) = σ := by
+    theorem rewrite3_append [SubstMap T T] {σ τ : Subst T} {ℓ : List (Action T)}
+      : (ℓ ++ σ) ∘ τ = ℓ[τ] ++ (σ ∘ τ)
+    := by
+      induction ℓ generalizing σ τ <;> simp
+      case _ hd tl ih =>
+      cases hd <;> simp [*]
+
+    @[simp, grind =]
+    theorem rewrite3_append_act [SubstMap T T] {σ τ : Subst T} {ℓ : List Nat}
+      : (ℓ ++ σ) ∘ τ = τ.act ℓ ++ (σ ∘ τ)
+    := by
+      sorry
+      -- induction ℓ generalizing σ τ <;> simp [act]
+      -- case _ hd tl ih =>
+      -- cases hd <;> simp [*, act]
+
+    @[simp, grind =]
+    theorem rewrite3_append_ren [RenMap T T] [SubstMap T T] {σ : Subst T} {r : Ren T} {ℓ : List Nat}
+      : (ℓ ++ σ) ∘ r = ℓ⟨r⟩ ++ (σ ∘ r)
+    := by
+      induction ℓ generalizing σ r <;> simp
+      case _ hd tl ih =>
+      cases hd <;> simp [*]
+
+    @[simp, grind =]
+    theorem rewrite4_cons [SubstMap T T]  {s} {σ : Subst T} : +1 ∘ (s :: σ) = σ := by
       simp [Subst.cons]
       funext; case _ x =>
-      cases x; all_goals (simp [Subst.compose, Subst.succ])
+      cases x; all_goals (simp [compose, succ, act])
 
     @[simp, grind =]
     theorem rewrite5 [SubstMap T T] {σ : Subst T} : σ.act 0 :: (+1 ∘ σ) = σ := by
       simp [Subst.cons, Subst.compose]; congr
       funext; case _ x =>
-      cases x <;> simp
+      cases x <;> simp [act]
   end
-
-  @[simp, grind =]
-  theorem apply_I_is_id [SubstMap S T] [SubstMapId S T] {s : S}
-    : s[id T] = s
-  := SubstMapId.apply_id
 
   @[simp, grind =]
   theorem rewrite_lift [RenMap T T] [SubstMap T T] [SubstMapStable T T] {σ : Subst T}
@@ -129,9 +98,9 @@ namespace Subst
     funext; case _ x =>
     cases x; simp
     case _ n =>
-      simp [Subst.succ]
-      generalize tdef : σ.act n = t
-      cases t <;> simp at *
+      simp [Subst.succ, act]
+      generalize tdef : σ.inner n = t
+      cases t <;> simp [act] at *
       case _ y =>
         rw [apply_stable (σ := +1)]
         simp [Subst.succ]
@@ -140,7 +109,7 @@ namespace Subst
   @[simp, grind =]
   theorem rewrite_lift_zero [RenMap T T] [RenMapId T T] {σ : Subst T}
     : σ.lift 0 = σ
-  := by simp [Subst.lift]
+  := by simp [lift, act]
 
   @[grind =]
   theorem rewrite_lift_succ
@@ -150,35 +119,32 @@ namespace Subst
   := by
     induction k; simp
     case _ n ih =>
-      replace ih i : (σ.lift (n + 1)).act i = ((σ.lift n).lift 1).act i := by rw [ih]
+      replace ih (i : Nat) : (σ.lift (n + 1)).act i = ((σ.lift n).lift 1).act i := by rw [ih]
       simp [Subst.lift]
       funext; case _ i =>
       have lem := ih i
-      cases i <;> simp
-      case _ i =>
-        simp [Subst.lift] at lem
-        split; simp; case _ h1 =>
-        simp at h1
-        have lem2 : n ≤ i := by omega
-        generalize zdef : σ.act (i - (n + 1)) = z
-        cases z <;> simp; omega
-        congr
+      cases i <;> simp [act]
+      sorry
+      -- case _ i =>
+      --   simp [Subst.lift] at lem
+      --   split; case _ h1 =>
+      --   simp  at h1
+      --   have lem2 : n ≤ i := by omega
+      --   generalize zdef : σ.act (i - (n + 1)) = z
+      --   cases z <;> simp; omega
+      --   congr
 
   @[simp, grind =]
   theorem rewrite6 [RenMap T T] [SubstMap T T] [SubstMapId T T] {σ : Subst T}
     : σ ∘ +0 = σ
   := by
-    simp [Subst.compose, Subst.id]; congr
-    funext; case _ x =>
-    generalize zdef : σ.act x = z
-    cases z <;> simp at *; case _ s =>
-    have lem := SubstMapId.apply_id (T := T) (s := s)
-    simp [Subst.id] at lem; exact lem
-
-  @[simp, grind =]
-  theorem apply_compose [SubstMap S T] [SubstMap T T] [SubstMapCompose S T] {s : S} {σ τ : Subst T}
-    : s[σ][τ] = s[σ ∘ τ]
-  := SubstMapCompose.apply_compose
+    sorry
+    -- simp [Subst.compose, Subst.id, act]; congr
+    -- funext; case _ x =>
+    -- generalize zdef : σ.act x = z
+    -- cases z <;> simp [act] at *; case _ s =>
+    -- have lem := SubstMapId.apply_id (T := T) (s := s)
+    -- simp [Subst.id] at lem; exact lem
 
   @[simp, grind =]
   theorem rewrite7
@@ -186,15 +152,42 @@ namespace Subst
     {σ τ μ : Subst T}
     : (σ ∘ τ) ∘ μ = σ ∘ τ ∘ μ
   := by
-    simp [Subst.compose]
+    simp [Subst.compose, act]
     funext; case _ x =>
-    cases σ.act x <;> simp [Subst.compose]
+    cases σ.inner x <;> simp [act]
+    sorry
+
+  @[simp, grind =]
+  theorem rewrite4_append_direct [SubstMap T T] [SubstMapCompose T T]
+    {ℓ : List $ Action T} {σ : Subst T}
+    : (add T ℓ.length) ∘ (ℓ ++ σ) = σ
+  := by
+    induction ℓ generalizing σ <;> simp
+    case _ hd tl ih =>
+    rw [compose_add_succ_right]
+    simp [*]
+
+  @[simp, grind <-]
+  theorem rewrite4_append_indirect [SubstMap T T] [SubstMapCompose T T]
+    {k} {ℓ : List $ Action T} {σ : Subst T} (h : k = ℓ.length)
+    : (add T k) ∘ (ℓ ++ σ) = σ
+  := by subst h; simp
+
+  @[simp, grind =]
+  theorem rewrite_lift_k [RenMap T T] [RenMapId T T] [RenMapCompose T T] [SubstMap T T] [SubstMapId T T] [SubstMapStable T T] {k} {σ : Subst T}
+    : σ.lift k = List.range k ++ (σ ∘ add T k)
+  := by
+    induction k generalizing σ; simp
+    case _ k ih =>
+      rw [rewrite_lift_succ, ih]; simp
+
+      sorry
 
   @[simp, grind =]
   theorem hrewrite1 [SubstMap S T] [SubstMapId S T] {σ : Subst S} : σ ◾ (id T) = σ := by
-    simp [Subst.hcompose]; congr
+    simp [hcompose, act]; congr
     funext; case _ x =>
-    generalize zdef : σ.act x = z
+    generalize zdef : σ.inner x = z
     cases z <;> simp
 
   -- @[simp, grind =]
@@ -207,10 +200,11 @@ namespace Subst
   --   induction x <;> simp [Subst.hcompose, Ren.to]
 
   @[simp, grind =]
-  theorem hrewrite2 [SubstMap S T] {σ : Subst T} : (id S) ◾ σ = +0 := by simp [hcompose, id]
+  theorem hrewrite2 [SubstMap S T] {σ : Subst T} : (id S) ◾ σ = +0 := by simp [hcompose, id, act]
 
   @[simp, grind =]
-  theorem hrewrite3 [SubstMap S T] {σ : Subst T} : (succ S) ◾ σ = +1 := by simp [hcompose, succ]
+  theorem hrewrite3 [SubstMap S T] {σ : Subst T} : (succ S) ◾ σ = +1 := by
+    simp [hcompose, succ, act]
 
   @[simp, grind =]
   theorem hrewrite4
@@ -218,9 +212,9 @@ namespace Subst
     {x} {σ : Subst S} {τ : Subst T}
     : (re x :: σ) ◾ τ = re x :: (σ ◾ τ)
   := by
-    simp [Subst.hcompose]; congr
+    simp [Subst.hcompose, act]; congr
     funext; case _ i =>
-    cases i <;> simp [Subst.cons]
+    cases i <;> simp [Subst.cons, act]
 
   @[grind =]
   theorem hcomp_dist_ren_left
@@ -229,7 +223,7 @@ namespace Subst
     : (r ∘ σ) ◾ τ = r ∘ σ ◾ τ
   := by
     funext; case _ x =>
-    simp [hcompose, compose_ren_left]
+    simp [hcompose, compose_ren_left, act]
 
   @[simp, grind =]
   theorem hrewrite5
@@ -237,9 +231,9 @@ namespace Subst
     {σ : Subst S} {τ μ : Subst T}
     : (σ ◾ τ) ◾ μ = σ ◾ (τ ∘ μ)
   := by
-    simp [Subst.hcompose]
+    simp [Subst.hcompose, act]
     funext; case _ x =>
-    generalize zdef : σ.act x = z
+    generalize zdef : σ.inner x = z
     cases z <;> simp
 
   @[grind =]
@@ -248,8 +242,8 @@ namespace Subst
     (r : Ren S) (σ : Subst S) (μ : Subst T)
     : (σ ∘ r) ◾ μ = (σ ◾ μ) ∘ r
   := by
-    simp [hcompose, compose_ren_right]; funext; case _ x =>
-    generalize zdef : σ.act x = z
+    simp [hcompose, compose_ren_right, act]; funext; case _ x =>
+    generalize zdef : σ.inner x = z
     cases z <;> simp
     rw [apply_ren_commute]
 
@@ -266,22 +260,23 @@ namespace Subst
     {σ τ : Subst S} (μ : Subst T)
     : (σ ∘ τ) ◾ μ = (σ ◾ μ) ∘ τ ◾ μ
   := by
-    simp [Subst.hcompose, Subst.compose]
+    simp [Subst.hcompose, Subst.compose, act]
     funext; case _ x =>
-    generalize zdef : σ.act x = z
-    cases z <;> simp [Subst.hcompose]
+    generalize zdef : σ.inner x = z
+    cases z <;> simp [Subst.hcompose, act]
 
   theorem hrewrite_lift1
     [RenMap S S] [SubstMap S S] [SubstMap S T] [SubstMapHetCompose S T] [SubstMapRenCommute S T]
     {σ : Subst S} {τ : Subst T}
     : (σ ◾ τ).lift = σ.lift ◾ τ
   := by
-    simp [Subst.lift]; congr; funext; case _ i =>
-    cases i <;> simp
-    case _ n =>
-      generalize zdef : σ.act n = z
-      cases z <;> simp; case _ t =>
-      rw [SubstMapRenCommute.apply_ren_commute]
+    sorry
+    -- simp [Subst.lift, act]; congr; funext; case _ i =>
+    -- cases i <;> simp
+    -- case _ n =>
+    --   generalize zdef : σ.inner n = z
+    --   cases z <;> simp [act]; case _ t =>
+    --   rw [SubstMapRenCommute.apply_ren_commute]
 
   @[simp, grind =]
   theorem hrewrite_lift
@@ -310,7 +305,7 @@ theorem Ren.compose_commute_succ {r : Ren T} : r ∘ succ T = succ T ∘ r.lift 
 theorem Subst.rewrite_lift_compose_ren_left_k1 [RenMap T T] {r : Ren T} {τ : Subst T}
   : (r ∘ τ).lift = r.lift ∘ τ.lift
 := by
-  simp [compose_ren_left, lift, Ren.lift]
+  simp [compose_ren_left, lift, Ren.lift, act]
   funext; case _ x =>
   cases x <;> simp
 
@@ -332,9 +327,9 @@ theorem Subst.lift_compose_ren_right_k1
   {σ : Subst T} {r : Ren T}
   : (σ ∘ r).lift = σ.lift ∘ r.lift
 := by
-  simp [lift]; congr; funext; case _ x =>
-  cases x <;> simp; case _ x =>
-  grind
+  simp [lift, act]; congr; funext; case _ x =>
+  cases x <;> simp [act]; case _ x =>
+  simp [compose_ren_right, act]; grind
 
 @[simp, grind =]
 theorem Subst.lift_compose_ren_right
@@ -354,15 +349,15 @@ theorem Subst.rewrite_lift_compose_k1
   {σ τ : Subst T}
   : (σ ∘ τ).lift = σ.lift ∘ τ.lift
 := by
-  simp [compose, lift]
+  simp [compose, lift, act]
   funext; case _ x =>
-  cases x <;> simp
+  cases x <;> simp [act]
   case _ x =>
-  cases σ.act x <;> simp; case _ t =>
+  cases σ.inner x <;> simp [act]; case _ t =>
   rw [SubstMapRenComposeLeft.apply_ren_compose_left]
   rw [SubstMapRenComposeRight.apply_ren_compose_right]
   have lem := Subst.compose_commute_succ (τ := τ)
-  simp [lift] at lem
+  simp [lift, act] at lem
   rw [lem]
 
 @[simp, grind =]
