LeanSubst/Ops.lean
@@ -70,7 +70,7 @@ theorem Action.hsmap_re [SubstMap S T] {σ : Subst T} {x : Nat} : (@re S x)[σ] 
   simp [SubstMap.smap]
 
 @[simp]
-theorem Actionh.smap_su [SubstMap S T] {σ : Subst T} {t : S} : (su t)[σ] = su t[σ] := by
+theorem Action.hsmap_su [SubstMap S T] {σ : Subst T} {t : S} : (su t)[σ] = su t[σ] := by
   simp [SubstMap.smap]
 ----------------------------------------------------------------------------------------------------
 ---- Identity
@@ -78,39 +78,39 @@ theorem Actionh.smap_su [SubstMap S T] {σ : Subst T} {t : S} : (su t)[σ] = su 
 def Ren.id T : Ren T := ⟨λ x => x⟩
 
 @[simp]
-theorem Ren.id_action {x} : (id T).act x = x := by simp [Ren.id]
+theorem Ren.id_action {x} : (id T).act x = x := by simp [id]
 
 def Subst.id T : Subst T := ⟨λ x => re x⟩
 notation "+0" => Subst.id _
 
 @[simp]
-theorem Subst.id_action {x} : (id T).act x = re x := by simp [Subst.id]
+theorem Subst.id_action {x} : (id T).act x = re x := by simp [id, act]
 ----------------------------------------------------------------------------------------------------
 ---- Successor
 ----------------------------------------------------------------------------------------------------
 def Ren.succ T : Ren T := ⟨(· + 1)⟩
 
 @[simp]
-theorem Ren.succ_action {x} : (succ T).act x = x + 1 := by simp [Ren.succ]
+theorem Ren.succ_action {x} : (succ T).act x = x + 1 := by simp [succ]
 
 def Subst.succ T : Subst T := ⟨λ x => re $ x + 1⟩
 notation "+1" => Subst.succ _
 
 @[simp]
-theorem Subst.succ_action {x} : (succ T).act x = re (x + 1) := by simp [Subst.succ]
+theorem Subst.succ_action {x} : (succ T).act x = re (x + 1) := by simp [succ, act]
 ----------------------------------------------------------------------------------------------------
 ---- Predecessor
 ----------------------------------------------------------------------------------------------------
 def Ren.pred T : Ren T := ⟨(· - 1)⟩
 
 @[simp]
-theorem Ren.pred_action {x} : (pred T).act x = x - 1 := by simp [Ren.pred]
+theorem Ren.pred_action {x} : (pred T).act x = x - 1 := by simp [pred]
 
 def Subst.pred T : Subst T := ⟨λ x => re $ x - 1⟩
 notation "-1" => Subst.pred _
 
 @[simp]
-theorem Subst.pred_action {x} : (pred T).act x = re (x - 1) := by simp [Subst.pred]
+theorem Subst.pred_action {x} : (pred T).act x = re (x - 1) := by simp [pred, act]
 ----------------------------------------------------------------------------------------------------
 ---- Addition
 ----------------------------------------------------------------------------------------------------
@@ -128,37 +128,37 @@ theorem Ren.add_one : add T 1 = succ T := by simp [Ren.add, Ren.succ]
 def Subst.add T (k : Nat) : Subst T := ⟨λ x => re $ x + k⟩
 
 @[simp]
-theorem Subst.add_action {k x} : (add T k).act x = re (x + k) := by simp [Subst.add]
+theorem Subst.add_action {k x} : (add T k).act x = re (x + k) := by simp [add, act]
 
 @[simp]
-theorem Subst.add_zero : add T 0 = +0 := by simp [Subst.add, Subst.id]
+theorem Subst.add_zero : add T 0 = +0 := by simp [add, id]
 
 @[simp]
-theorem Subst.add_one : add T 1 = +1 := by simp [Subst.add, Subst.succ]
+theorem Subst.add_one : add T 1 = +1 := by simp [add, succ]
 ----------------------------------------------------------------------------------------------------
 ---- Subtraction
 ----------------------------------------------------------------------------------------------------
 def Ren.sub T (k : Nat) : Ren T := ⟨(· - k)⟩
 
 @[simp]
-theorem Ren.sub_action {k x} : (sub T k).act x = x - k := by simp [Ren.sub]
+theorem Ren.sub_action {k x} : (sub T k).act x = x - k := by simp [sub]
 
 @[simp]
-theorem Ren.sub_zero : sub T 0 = id T := by simp [Ren.sub, Ren.id]
+theorem Ren.sub_zero : sub T 0 = id T := by simp [sub, id]
 
 @[simp]
-theorem Ren.sub_one : sub T 1 = pred T := by simp [Ren.sub, Ren.pred]
+theorem Ren.sub_one : sub T 1 = pred T := by simp [sub, pred]
 
 def Subst.sub T (k : Nat) : Subst T := ⟨λ x => re $ x - k⟩
 
 @[simp]
-theorem Subst.sub_action {k x} : (@sub T k).act x = re (x - k) := by simp [Subst.sub]
+theorem Subst.sub_action {k x} : (@sub T k).act x = re (x - k) := by simp [sub, act]
 
 @[simp]
-theorem Subst.sub_zero : sub T 0 = +0 := by simp [Subst.sub, Subst.id]
+theorem Subst.sub_zero : sub T 0 = +0 := by simp [sub, id]
 
 @[simp]
-theorem Subst.sub_one : sub T 1 = -1 := by simp [Subst.sub, Subst.pred]
+theorem Subst.sub_one : sub T 1 = -1 := by simp [sub, pred]
 
 ----------------------------------------------------------------------------------------------------
 ---- Cons
@@ -170,10 +170,10 @@ def Ren.cons (a : Nat) (r : Ren T) : Ren T := .mk λ n =>
 infixr:67 (name := Ren.cons_notation) " :: " => Ren.cons
 
 @[simp]
-theorem Ren.cons_action0 {a} {r : Ren T} : (a::r).act 0 = a := by simp [Ren.cons]
+theorem Ren.cons_action0 {a} {r : Ren T} : (a::r).act 0 = a := by simp [cons]
 
 @[simp]
-theorem Ren.cons_action {a i} {r : Ren T} : (a::r).act (i + 1) = r.act i := by simp [Ren.cons]
+theorem Ren.cons_action {a i} {r : Ren T} : (a::r).act (i + 1) = r.act i := by simp [cons]
 
 def Subst.cons (a : Action T) (σ : Subst T) : Subst T := .mk λ n =>
   match n with
@@ -182,10 +182,10 @@ def Subst.cons (a : Action T) (σ : Subst T) : Subst T := .mk λ n =>
 infixr:67 (name := Subst.cons_notation) " :: " => Subst.cons
 
 @[simp]
-theorem Subst.cons_action0 {a} {σ : Subst T} : (a::σ).act 0 = a := by simp [Subst.cons]
+theorem Subst.cons_action0 {a} {σ : Subst T} : (a::σ).act 0 = a := by simp [cons, act]
 
 @[simp]
-theorem Subst.cons_action {a i} {σ : Subst T} : (a::σ).act (i + 1) = σ.act i := by simp [Subst.cons]
+theorem Subst.cons_action {a i} {σ : Subst T} : (a::σ).act (i + 1) = σ.act i := by simp [cons, act]
 ----------------------------------------------------------------------------------------------------
 ---- Append
 ----------------------------------------------------------------------------------------------------
@@ -198,11 +198,11 @@ instance : HAppend (List Nat) (Ren T) (Ren T) where
 
 @[simp]
 theorem Ren.append_nil {r : Ren T} : ([] : List Nat) ++ r = r := by
-  simp [HAppend.hAppend, Ren.append]
+  simp [HAppend.hAppend, append]
 
 @[simp]
 theorem Ren.append_cons {a} {ℓ : List Nat} {r : Ren T} : (a::ℓ) ++ r = a::(ℓ ++ r) := by
-  simp [HAppend.hAppend, Ren.append]
+  simp [HAppend.hAppend, append]
 
 @[simp, grind <-]
 theorem Ren.append_action_lt {r : Ren T} {i}
@@ -230,11 +230,11 @@ instance : HAppend (List $ Action T) (Subst T) (Subst T) where
 
 @[simp]
 theorem Subst.append_nil {σ : Subst T} : ([] : List $ Action T) ++ σ = σ := by
-  simp [HAppend.hAppend, Subst.append]
+  simp [HAppend.hAppend, append]
 
 @[simp]
 theorem Subst.append_cons {a} {ℓ : List $ Action T} {σ : Subst T} : (a::ℓ) ++ σ = a::(ℓ ++ σ) := by
-  simp [HAppend.hAppend, Subst.append]
+  simp [HAppend.hAppend, append]
 
 @[simp, grind <-]
 theorem Subst.append_action_lt {σ : Subst T} {i}
@@ -252,6 +252,38 @@ theorem Subst.append_action_ge {σ : Subst T} {i}
   match i with
   | 0 => by simp at h
   | i + 1 => @append_action_ge σ i tl (by grind) |> cast (by simp)
+
+def Subst.append_ren : List Nat -> Subst T -> Subst T
+| .nil, r => r
+| .cons hd tl, r => re hd::append_ren tl r
+
+instance : HAppend (List Nat) (Subst T) (Subst T) where
+  hAppend := Subst.append_ren
+
+@[simp]
+theorem Subst.append_ren_nil {σ : Subst T} : ([] : List $ Nat) ++ σ = σ := by
+  simp [HAppend.hAppend, append_ren]
+
+@[simp]
+theorem Subst.append_ren_cons {a} {ℓ : List Nat} {σ : Subst T} : (a::ℓ) ++ σ = re a::(ℓ ++ σ) := by
+  simp [HAppend.hAppend, append_ren]
+
+@[simp, grind <-]
+theorem Subst.append_ren_action_lt {σ : Subst T} {i}
+  : {ℓ : List Nat} -> (h : i < ℓ.length) -> (ℓ ++ σ).act i = re ℓ[i]
+| .cons hd tl, h =>
+  match i with
+  | 0 => rfl
+  | i + 1 => append_ren_action_lt (σ := σ) (ℓ := tl) (by grind)
+
+@[simp, grind <-]
+theorem Subst.append_ren_action_ge {σ : Subst T} {i}
+  : {ℓ : List Nat} -> (h : i ≥ ℓ.length) -> (ℓ ++ σ).act i = σ.act (i - ℓ.length)
+| .nil, h => by simp
+| .cons hd tl, h =>
+  match i with
+  | 0 => by simp at h
+  | i + 1 => @append_ren_action_ge σ i tl (by grind) |> cast (by simp)
 ----------------------------------------------------------------------------------------------------
 ---- Composition
 ----------------------------------------------------------------------------------------------------
@@ -260,20 +292,17 @@ def Ren.compose : Ren T -> Ren T -> Ren T
 infixr:85 " ∘ " => Ren.compose
 
 @[simp]
-theorem Ren.compose_action {r1 r2 : Ren T} {x} : (r1 ∘ r2).act x = r2.act (r1.act x) :=
-  by simp [Ren.compose]
+theorem Ren.compose_action {r1 r2 : Ren T} {x} : (r1 ∘ r2).act x = r2.act (r1.act x) := by
+  simp [compose]
 
 @[simp]
-theorem Ren.compose_id_left {r : Ren T} : id T ∘ r = r := by
-  simp [Ren.compose, Ren.id]
+theorem Ren.compose_id_left {r : Ren T} : id T ∘ r = r := by simp [compose, id]
 
 @[simp]
-theorem Ren.compose_id_right {r : Ren T} : r ∘ id T = r := by
-  simp [Ren.compose, Ren.id]
+theorem Ren.compose_id_right {r : Ren T} : r ∘ id T = r := by simp [compose, id]
 
 @[simp]
-theorem Ren.compose_assoc {r1 r2 r3 : Ren T} : (r1 ∘ r2) ∘ r3 = r1 ∘ r2 ∘ r3 := by
-  simp [Ren.compose]
+theorem Ren.compose_assoc {r1 r2 r3 : Ren T} : (r1 ∘ r2) ∘ r3 = r1 ∘ r2 ∘ r3 := by simp [compose]
 
 @[simp]
 theorem Ren.compose_pred_succ : succ T ∘ pred T = id T := by simp [succ, pred, id, compose]
@@ -281,34 +310,38 @@ theorem Ren.compose_pred_succ : succ T ∘ pred T = id T := by simp [succ, pred,
 @[simp]
 theorem Ren.compose_sub_add {k} : add T k ∘ sub T k = id T := by simp [sub, add, id, compose]
 
--- -- r1 contains only S-vars, hence a renaming of T-vars is a no-op
--- def Ren.hcompose : Ren S -> Ren T -> Ren S
--- | r, _ => .mk λ n => r.act n
--- infixr:85 " ◾ " => Ren.hcompose
+@[grind =]
+theorem Ren.compose_add_succ_right {k} : add T (k + 1) = add T k ∘ succ T := by
+  simp [add, succ, compose]; grind
 
--- @[simp]
--- theorem Ren.hcompose_ext {r1 : Ren S} {r2 : Ren T} : r1 ◾ r2 = r1 := sorry
-
--- -- same deal as `Ren.hcompose`
--- def Ren.hcompose_subst : Ren S -> Subst T -> Ren S
--- | r, _ => .mk λ n => r.act n
--- infixr:85 " ◾ " => Ren.hcompose
+@[grind =]
+theorem Ren.compose_add_succ_left {k} : add T (k + 1) = succ T ∘ add T k := by
+  simp [add, succ, compose]; grind
 
 def Subst.compose [SubstMap T T] : Subst T -> Subst T -> Subst T
 | σ, τ => .mk λ n => (σ.act n)[τ]
 infixr:85 (name := Subst.compose_notation) " ∘ " => Subst.compose
 
 @[simp]
-theorem Subst.compose_action [SubstMap T T] {σ τ : Subst T} {x} : (σ ∘ τ).act x = (σ.act x)[τ] := by
-  simp [Subst.compose]
+theorem Subst.compose_action [SubstMap T T] {σ τ : Subst T} {x : Nat}
+  : (σ ∘ τ).act x = (σ.act x)[τ]
+:= by simp [compose, act]
 
 @[simp]
 theorem Subst.compose_pred_succ [SubstMap T T] : succ T ∘ pred T = id T := by
-  simp [succ, pred, id, compose]
+  simp [succ, pred, id, compose, act]
 
 @[simp]
 theorem Subst.compose_sub_add [SubstMap T T] {k} : add T k ∘ sub T k = id T := by
-  simp [sub, add, id, compose]
+  simp [sub, add, id, compose, act]
+
+@[grind =]
+theorem Subst.compose_add_succ_right [SubstMap T T] {k} : add T (k + 1) = add T k ∘ succ T := by
+  simp [add, succ, compose, act]; grind
+
+@[grind =]
+theorem Subst.compose_add_succ_left [SubstMap T T] {k} : add T (k + 1) = succ T ∘ add T k := by
+  simp [add, succ, compose, act]; grind
 
 def Subst.compose_ren_left : Ren T -> Subst T -> Subst T
 | r, τ => .mk λ n => τ.act (r.act n)
@@ -317,34 +350,34 @@ infixr:85 (name := Subst.compose_ren_left_notation) " ∘ " => Subst.compose_ren
 @[simp]
 theorem Subst.compose_ren_left_action {r : Ren T} {τ : Subst T} {x}
   : (r ∘ τ).act x = τ.act (r.act x)
-:= by simp [Subst.compose_ren_left]
+:= by simp [compose_ren_left, act]
 
 def Subst.compose_ren_right [RenMap T T] : Subst T -> Ren T -> Subst T
 | σ, r => .mk λ n => (σ.act n)⟨r⟩
 infixr:85 (name := Subst.compose_ren_right_notation) " ∘ " => Subst.compose_ren_right
 
 @[simp]
-theorem Subst.compose_ren_right_action [RenMap T T] {σ : Subst T} {r : Ren T} {x}
+theorem Subst.compose_ren_right_action [RenMap T T] {σ : Subst T} {r : Ren T} {x : Nat}
   : (σ ∘ r).act x = (σ.act x)⟨r⟩
-:= by simp [Subst.compose_ren_right]
+:= by simp [compose_ren_right, act]
 
 def Subst.hcompose [SubstMap S T] : Subst S -> Subst T -> Subst S
 | σ, τ => .mk λ n => (σ.act n)[τ]
 infixr:85 " ◾ " => Subst.hcompose
 
 @[simp]
-theorem Subst.hcompose_action [SubstMap S T] {σ : Subst S} {τ : Subst T} {x}
+theorem Subst.hcompose_action [SubstMap S T] {σ : Subst S} {τ : Subst T} {x : Nat}
   : (σ ◾ τ).act x = (σ.act x)[τ]
-:= by simp [Subst.hcompose]
+:= by simp [hcompose, act]
 
 def Subst.hcompose_ren [RenMap S T] : Subst S -> Ren T -> Subst S
 | σ, r => .mk λ n => (σ.act n)⟨r⟩
 infixr:85 " ◾ " => Subst.hcompose_ren
 
 @[simp]
-theorem Subst.hcompose_ren_action [RenMap S T] {σ : Subst S} {r : Ren T} {x}
+theorem Subst.hcompose_ren_action [RenMap S T] {σ : Subst S} {r : Ren T} {x : Nat}
   : (σ ◾ r).act x = (σ.act x)⟨r⟩
-:= by simp [Subst.hcompose_ren]
+:= by simp [hcompose_ren, act]
 
 ----------------------------------------------------------------------------------------------------
 ---- Lift
@@ -354,11 +387,11 @@ def Ren.lift (r : Ren T) (k : Nat := 1) : Ren T := .mk λ n =>
 
 @[simp, grind <-]
 theorem Ren.lift_action_lt {r : Ren T} {k i} (h : i < k) : (lift r k).act i = i := by
-  simp [Ren.lift]; grind
+  simp [lift]; grind
 
 @[simp, grind <-]
 theorem Ren.lift_action_ge {r : Ren T} {k i} (h : i ≥ k) : (lift r k).act i = r.act (i - k) + k :=
-  by simp [Ren.lift]; grind
+  by simp [lift]; grind
 
 @[simp]
 theorem Ren.lift_of_zero {r : Ren T} : r.lift 0 = r := by
@@ -374,11 +407,11 @@ theorem Ren.lift_of_succ {r : Ren T} {k} : r.lift (k + 1) = (r.lift k).lift := b
 
 @[simp]
 theorem Ren.lift_id {k} : lift (id T) k = id T := by
-  simp [Ren.id, Ren.lift]; congr; funext; case _ x =>
+  simp [id, lift]; congr; funext; case _ x =>
   cases x <;> simp; omega
 
 theorem Ren.lift_compose1 {r1 r2 : Ren T} : (r1 ∘ r2).lift = r1.lift ∘ r2.lift := by
-  simp [Ren.compose, Ren.lift]
+  simp [compose, lift]
   funext; case _ x =>
   cases x <;> simp
 
@@ -397,19 +430,40 @@ def Subst.lift [RenMap T T] (σ : Subst T) (k : Nat := 1) : Subst T := .mk λ n 
 @[simp, grind <-]
 theorem Subst.lift_action_lt [RenMap T T] {σ : Subst T} {k i} (h : i < k)
   : (lift σ k).act i = re i
-:= by simp [Subst.lift]; grind
+:= by simp [lift, act]; grind
 
 @[simp, grind <-]
 theorem Subst.lift_action_ge [RenMap T T] {σ : Subst T} {k i} (h : i ≥ k)
   : (lift σ k).act i = (σ.act (i - k))⟨.add T k⟩
-:= by simp [Subst.lift]; grind
+:= by simp [lift, act]; grind
+----------------------------------------------------------------------------------------------------
+---- Action on variable list
+----------------------------------------------------------------------------------------------------
+def Subst.act_list (σ : Subst T) : (ℓ : List Nat) -> List (Action T)
+| [] => []
+| .cons x xs => σ.act x :: act_list σ xs
+
+instance : SubstAction T (List Nat) (List (Action T)) where
+  act := Subst.act_list
+
+@[simp]
+theorem Subst.act_list_nil {σ : Subst T} : σ.act ([] : List Nat) = [] := by simp [act_list, act]
+
+@[simp]
+theorem Subst.act_list_cons {σ : Subst T} {x} {ℓ : List Nat} : σ.act (x::ℓ) = σ.act x :: σ.act ℓ :=
+  by simp [act_list, act]
+
+@[simp]
+theorem Subst.act_list_append {σ : Subst T} {x y : List Nat}
+  : σ.act (x ++ y) = σ.act x ++ σ.act y
+:= by induction x generalizing y <;> simp [*]
 ----------------------------------------------------------------------------------------------------
 ---- Promotion
 ----------------------------------------------------------------------------------------------------
 def Ren.to (r : Ren T) : Subst T := ⟨λ x => re (r.act x)⟩
 
 @[simp]
-theorem Ren.to_act {r : Ren T} {x} : (@to T r).act x = re (r.act x) := by simp [Ren.to]
+theorem Ren.to_act {r : Ren T} {x} : (@to T r).act x = re (r.act x) := by simp [to, SubstAction.act]
 
 @[simp]
 theorem Ren.to_id : (id T).to = .id T := by simp [to, id, Subst.id]
@@ -428,7 +482,7 @@ theorem Ren.to_sub {k} : (sub T k).to = .sub T k := by simp [to, sub, Subst.sub]
 
 @[simp]
 theorem Ren.to_lift [RenMap T T] {r : Ren T} {k} : (r.lift k).to = (@to T r).lift k := by
-  cases r; simp [to, lift, Subst.lift]; case _ act =>
+  cases r; simp [to, lift, Subst.lift, SubstAction.act]; case _ act =>
   funext; case _ x =>
   cases x; grind
   case _ n => cases Nat.decLt (n + 1) k <;> simp [ite]
@@ -438,6 +492,6 @@ theorem Ren.to_compose [RenMap T T] [SubstMap T T] {r1 r2 : Ren T}
   : @to T (r1 ∘ r2) = r1.to ∘ r2.to
 := by
   funext; case _ x =>
-  cases x <;> simp [to, compose, Subst.compose]
+  cases x <;> simp [to, compose, Subst.compose, SubstAction.act]
 
 end LeanSubst
