LeanSubst/Class.lean
@@ -1,0 +1,72 @@
+import LeanSubst.Basic
+import LeanSubst.Ops
+
+namespace LeanSubst
+
+universe u1 u2 u3
+variable {S : Type u1} {T : Type u2} {U : Type u3}
+
+class RenMapId (S : Type u1) (T : Type u2) [RenMap S T] where
+  apply_id {s : S} : s⟨.id T⟩ = s
+
+class RenMapCompose (S : Type u1) (T : Type u2) [RenMap S T] where
+  apply_compose {s : S} {r1 r2 : Ren T} : s⟨r1⟩⟨r2⟩ = s⟨r1 ∘ r2⟩
+
+@[simp]
+theorem Ren.apply_id [RenMap S T] [RenMapId S T] {s : S} : s⟨id T⟩ = s := RenMapId.apply_id
+
+@[simp, grind =]
+theorem Ren.apply_compose [RenMap S T] [RenMapCompose S T] {s : S} {r1 r2 : Ren T}
+  : s⟨r1⟩⟨r2⟩ = s⟨r1 ∘ r2⟩
+:= RenMapCompose.apply_compose
+
+instance (priority := high) [RenMap T T] [RenMapId T T] : RenMapId (Action T) T where
+  apply_id := by intro s; cases s <;> simp
+
+instance [RenMap S T] [RenMapId S T] : RenMapId (Action S) T where
+  apply_id := by intro s; cases s <;> simp
+
+instance (priority := high) [RenMap T T] [RenMapCompose T T] : RenMapCompose (Action T) T where
+  apply_compose := by intro s; cases s <;> simp
+
+instance [RenMap S T] [RenMapCompose S T] : RenMapCompose (Action S) T where
+  apply_compose := by intro s; cases s <;> simp
+
+class SubstMapId (S : Type u1) (T : Type u2) [SubstMap S T] where
+  apply_id {s : S} : s[.id T] = s
+
+class SubstMapStable (S : Type u1) (T : Type u2) [RenMap S T] [SubstMap S T] where
+  apply_stable (r : Ren T) (σ : Subst T) : r.to = σ -> rmap (S := S) r = smap σ
+
+class SubstMapRenComposeLeft (S : Type u1) (T : Type u2) [RenMap S T] [SubstMap S T] where
+  apply_ren_compose_left {s : S} {r : Ren T} {τ : Subst T} : s⟨r⟩[τ] = s[r ∘ τ]
+
+class SubstMapRenComposeRight (T : Type u2) [RenMap T T] [SubstMap T T] where
+  apply_ren_compose_right {t : T} {r : Ren T} {σ : Subst T} : t[σ]⟨r⟩ = t[σ ∘ r]
+
+class SubstMapCompose (S : Type u1) (T : Type u2) [SubstMap S T] [SubstMap T T] where
+  apply_compose {s : S} {σ τ : Subst T} : s[σ][τ] = s[σ ∘ τ]
+
+class SubstMapRenCommute (S : Type u1) (T : Type u2) [RenMap S S] [SubstMap S T] where
+  apply_ren_commute {s : S} (r : Ren S) (τ : Subst T) : s⟨r⟩[τ] = s[τ]⟨r⟩
+
+class SubstMapHetCompose (S : Type u1) (T : Type u2) [SubstMap S S] [SubstMap S T] where
+  apply_hcompose {s : S} {σ : Subst S} {τ : Subst T} : s[σ][τ] = s[τ][σ ◾ τ]
+
+namespace Subst
+  export SubstMapStable (apply_stable)
+  export SubstMapRenComposeLeft (apply_ren_compose_left)
+  export SubstMapRenComposeRight (apply_ren_compose_right)
+  export SubstMapRenCommute (apply_ren_commute)
+end Subst
+
+@[simp, grind =]
+theorem Subst.apply_id [SubstMap S T] [SubstMapId S T] {s : S} : s[.id T] = s := SubstMapId.apply_id
+
+@[simp, grind =]
+theorem Subst.apply_compose [SubstMap S T] [SubstMap T T] [SubstMapCompose S T]
+  {s : S} {σ τ : Subst T}
+  : s[σ][τ] = s[σ ∘ τ]
+:= SubstMapCompose.apply_compose
+
+end LeanSubst
