LeanSubst/Types/Nat.lean
@@ -1,0 +1,18 @@
+
+import LeanSubst.Class
+
+namespace LeanSubst
+
+universe u1 u2 u3
+variable {S : Type u1} {T : Type u2} {U : Type u3}
+
+def Nat.rmap (r : Ren T) : Nat -> Nat
+| n => r.act n
+
+instance : RenMap Nat T where
+  rmap := Nat.rmap
+
+@[simp, grind =]
+theorem Nat.rmap_simp {r : Ren T} {n} : n⟨r⟩ = r.act n := by simp [RenMap.rmap, Nat.rmap]
+
+end LeanSubst
